src/frontends/lean/elaborator.cpp
@@ -3507,7 +3507,7 @@ expr elaborator::visit_emptyc_or_emptys(expr const & e, optional<expr> const & e
         if (is_optional_param(new_expected_type))
             new_expected_type = app_arg(app_fn(new_expected_type));
         expr S = get_app_fn(new_expected_type);
-        if (is_constant(S) && is_structure(m_env, const_name(S))) {
+        if (is_constant(S) && const_name(S) != get_set_name() && is_structure(m_env, const_name(S))) {
             expr empty_struct = copy_tag(e, mk_structure_instance(name(), buffer<name>(), buffer<expr>()));
             return visit(empty_struct, expected_type);
         } else {
