src/library/constants.h
@@ -241,6 +241,7 @@ name const & get_reflected_subst_name();
 name const & get_repr_name();
 name const & get_rfl_name();
 name const & get_scope_trace_name();
+name const & get_set_name();
 name const & get_set_of_name();
 name const & get_sizeof_name();
 name const & get_string_name();
