library/init/data/set.lean
@@ -8,69 +8,54 @@ import init.meta.interactive
 import init.control.lawful
 
 universes u v
-def set (α : Type u) := α → Prop
 
-def set_of {α : Type u} (p : α → Prop) : set α :=
-p
+structure set (α : Type u) : Type u :=
+of :: (contains : α → Prop)
 
 namespace set
 variables {α : Type u} {β : Type v}
 
-protected def mem (a : α) (s : set α) :=
-s a
-
 instance : has_mem α (set α) :=
-⟨set.mem⟩
-
-protected def subset (s₁ s₂ : set α) :=
-∀ ⦃a⦄, a ∈ s₁ → a ∈ s₂
+⟨λ x s, s.contains x⟩
 
 instance : has_subset (set α) :=
-⟨set.subset⟩
-
-protected def sep (p : α → Prop) (s : set α) : set α :=
-{a | a ∈ s ∧ p a}
+⟨λ s₁ s₂, ∀ ⦃a⦄, a ∈ s₁ → a ∈ s₂⟩
 
 instance : has_sep α (set α) :=
-⟨set.sep⟩
+⟨λ p s, { a | a ∈ s ∧ p a}⟩
 
 instance : has_emptyc (set α) :=
-⟨λ a, false⟩
+⟨{ a | false }⟩
 
 def univ : set α :=
-λ a, true
-
-protected def insert (a : α) (s : set α) : set α :=
-{b | b = a ∨ b ∈ s}
+{ a | true }
 
 instance : has_insert α (set α) :=
-⟨set.insert⟩
+⟨λ a s, { b | b = a ∨ b ∈ s }⟩
 
-instance : has_singleton α (set α) := ⟨λ a, {b | b = a}⟩
+instance : has_singleton α (set α) := ⟨λ a, { b | b = a }⟩
+
+protected lemma ext {a b : set α} (h : ∀ x, x ∈ a ↔ x ∈ b) : a = b :=
+begin
+  cases a with a,
+  cases b with b,
+  simp [show a = b, from funext (λ x, propext (h _))]
+end
 
 instance : is_lawful_singleton α (set α) :=
-⟨λ a, funext $ λ b, propext $ or_false _⟩
-
-protected def union (s₁ s₂ : set α) : set α :=
-{a | a ∈ s₁ ∨ a ∈ s₂}
+⟨λ a, set.ext (λ x, or_false _)⟩
 
 instance : has_union (set α) :=
-⟨set.union⟩
-
-protected def inter (s₁ s₂ : set α) : set α :=
-{a | a ∈ s₁ ∧ a ∈ s₂}
+⟨λ s₁ s₂, { a | a ∈ s₁ ∨ a ∈ s₂ }⟩
 
 instance : has_inter (set α) :=
-⟨set.inter⟩
+⟨λ s₁ s₂, { a | a ∈ s₁ ∧ a ∈ s₂ }⟩
 
 def compl (s : set α) : set α :=
 {a | a ∉ s}
 
-protected def diff (s t : set α) : set α :=
-{a ∈ s | a ∉ t}
-
 instance : has_sdiff (set α) :=
-⟨set.diff⟩
+⟨λ s t, { a ∈ s | a ∉ t }⟩
 
 def powerset (s : set α) : set (set α) :=
 {t | t ⊆ s}
@@ -87,8 +72,8 @@ instance : functor set :=
 { map := @set.image }
 
 instance : is_lawful_functor set :=
-{ id_map := λ _ s, funext $ λ b, propext ⟨λ ⟨_, sb, rfl⟩, sb, λ sb, ⟨_, sb, rfl⟩⟩,
-  comp_map := λ _ _ _ g h s, funext $ λ c, propext
+{ id_map := λ _ s, set.ext $ λ b, ⟨λ ⟨_, sb, rfl⟩, sb, λ sb, ⟨_, sb, rfl⟩⟩,
+  comp_map := λ _ _ _ g h s, set.ext $ λ c,
     ⟨λ ⟨a, ⟨h₁, h₂⟩⟩, ⟨g a, ⟨⟨a, ⟨h₁, rfl⟩⟩, h₂⟩⟩,
      λ ⟨b, ⟨⟨a, ⟨h₁, h₂⟩⟩, h₃⟩⟩, ⟨a, ⟨h₁, by dsimp; cc⟩⟩⟩ }
 
