tests/lean/run/check_constants.lean
@@ -239,7 +239,8 @@ run_cmd script_check_id `reflected.subst
 run_cmd script_check_id `repr
 run_cmd script_check_id `rfl
 run_cmd script_check_id `scope_trace
-run_cmd script_check_id `set_of
+run_cmd script_check_id `set
+run_cmd script_check_id `set.of
 run_cmd script_check_id `sizeof
 run_cmd script_check_id `string
 run_cmd script_check_id `string.empty
